src/fem.h
@@ -1,7 +1,7 @@
 #ifndef FEM1D_H
 #define FEM1D_H
 #include "mesh.h"
-#include "assemble.h"
+#include "matrix.h"
 struct element_t;
 
 //ldoc on
@@ -92,17 +92,71 @@ void fem_set_load(fem_t fe, void (*f)(double* x, double* fx));
  * The following two functions need not be public except for unit tests;
  * normally they're called only from fem_assemble.
  */
-void assemble_matrix(assemble_t K, double* emat, int* ids, int ne);
+void assemble_matrix(matrix_t K, double* emat, int* ids, int ne);
 void assemble_vector(double* v, double* ve, int* ids, int ne);
 
 
 /**
+ * # Assembly
+ * 
+ * Each element in a finite element discretization consists of
+ * 
+ * - A domain $\Omega_e$ for the $e$th element, and
+ * - Local shape functions $N^e_1, \ldots, N^e_m$, which are often
+ *   Lagrange functions for interpolation at some set of nodes
+ *   in $\Omega_e$.
+ * 
+ * Each local shape function on the domain $\Omega_e$ is the
+ * restriction of some global shape function on the whole
+ * domain $\Omega$.  That is, we have global shape functions
+ * $$
+ *   N_{j}(x) = \sum_{j = \iota(j',e)} N^e_{j'}(x),
+ * $$
+ * where $\iota(j,e)$ denotes the mapping from the local shape
+ * function index for element $e$ to the corresponding global shape
+ * function index.  We only ever compute explicitly with the local
+ * functions $N^e_j$; the global functions are implicit.
+ * 
+ * *Assembly* is the process of reconstructing a quantity defined in
+ * terms of global shape functions from the contributions of the
+ * individual elements and their local shape functions.  For example,
+ * to compute
+ * $$
+ *   F_i = \int_{\Omega} f(x) N_i(x) \, dx,
+ * $$
+ * we rewrite the integral as
+ * $$
+ *   F_i = \sum_{i = \iota(i',e)} \int_{\Omega_e} f(x) N^e_{i'}(x) \, dx.
+ * $$
+ * In code, this is separated into two pieces:
+ * 
+ * - Compute element contributions $\int_{\Omega_e} f(x) N^e_{i'}(x) \, dx$.
+ *   This is the responsibility of the element implementation.
+ * - Sum contributions into the global position $i$ corresponding to
+ *   the element-local index $i'$.  This is managed by an assembly loop.
+ * 
+ * The concept of an "assembly loop" is central to finite element methods,
+ * but it is not unique to this setting.  For example, circuit simulators
+ * similarly construct system matrices (conductance, capacitance, etc)
+ * via the contributions of circuit elements (resistors, capacitors,
+ * inductors, and so forth).
+ * 
+ * We have two types of assembly loops that we care about: those that
+ * involve pairs of shape functions and result in matrices, and
+ * those that explicitly involve only a single shape function and result
+ * in vectors.
+ * 
+ * We will sometimes also want to discard some element contributions
+ * that correspond to interactions with shape functions associated with
+ * known boundary values (for example).  We also handle this filtering
+ * work as part of our assembly process.
+ * 
  * The assembly loops iterate through the elements and produce a global
  * residual and tangent stiffness based on the current solution state.
  * The residual and tangent matrix assembler are passed in by pointers;
  * a `NULL` pointer means "do not assemble this".
  */
-void fem_assemble(fem_t fe, double* R, assemble_t Kassembler);
+void fem_assemble(fem_t fe, double* R, matrix_t Kmatrix);
 void fem_assemble_band(fem_t fe, double* R, bandmat_t K);
 void fem_assemble_dense(fem_t fe, double* R, densemat_t K);
 
