src/matrix.h
@@ -1,0 +1,54 @@
+#ifndef ASSEMBLE_H
+#define ASSEMBLE_H
+#include <densemat.h>
+#include <bandmat.h>
+
+//ldoc on
+/**
+ * # Matrix interface
+ * 
+ * There are several matrix formats that we might want to use for
+ * solving the linear systems that arise from FEM problems.
+ * These include dense storage, banded storage, coordinate form, or CSR.  
+ * Because we would like
+ * to re-use the same FEM logic with these different formats,
+ * we define an abstract `assemble_t` interface with four basic methods:
+ * 
+ * - `add(m, i,j, x)` adds value x to the matrix component at (i,j)
+ * - `clear(m)` sets the matrix to zero, preserving the sparsity pattern ("graph").
+ * - `norm2(m)` returns the 2-norm (Frobenius norm) of the matrix
+ * - `print(m)` prints the matrix in some unspecified format
+ */
+
+// Interface for general assembler object (callback + context)
+typedef struct matrix_data_t *matrix_data_t;
+
+typedef struct matrix_t {
+    matrix_data_t p;                            // Context
+    void (*add)(matrix_data_t, int, int, double); // Add contribution
+    void (*clear)(matrix_data_t); // set to zero
+    double (*norm2)(matrix_data_t); // square of Frobenius norm
+    void (*print)(matrix_data_t);
+} *matrix_t;
+
+// Convenience functions that call the matrix methods
+void matrix_add(matrix_t m, int i, int j, double x);
+void matrix_clear(matrix_t m);
+double matrix_norm2(matrix_t m);
+void matrix_print(matrix_t m);
+
+/**
+ * We currently only support two types of matricess: dense and band.
+ * In all cases, we assume that the dimension `n` of the matrix
+ * is big enough (all active indices are less than `n`).  For the
+ * band matrix, we do NOT check to make sure there are no contributions
+ * that are outside the band; it's up to the client to establish that precondition.
+ *
+ * These functions leave the data (in the `A` or `b` argument) unchanged;
+ * if it was (partially) uninitialized before, so it remains.
+ */
+void init_matrix_dense(matrix_t m, densemat_t A);
+void init_matrix_band(matrix_t m, bandmat_t b);
+
+//ldoc off
+#endif /* ASSEMBLE_H */
